Fixed translation issues related to de Bruijn indices. Some progress in GRTT definitions: later_app and nextp

forcing/GRTT_SProp.v
@@ -4,7 +4,10 @@ Require Import String PeanoNat.
 Require Import Template.Checker.
 Require Import Template.Typing.
 Require Import Forcing.TemplateForcing.
+Require Import Forcing.translation_utils.
 Require Import List.
+
+Import ListNotations.
 
 (* Some axioms *)
 Require Import FunctionalExtensionality.
@@ -34,10 +37,15 @@ Proof.
   induction n;constructor;auto.
 Defined.
 
-Definition sle_S_eq {n m} : sle (S n) (S m) -> sle n m.
+Definition sle_Sn_Sm {n m} : sle (S n) (S m) -> sle n m.
 Proof.
   intros H.
   inversion H. apply ubox. subst. apply sbox. exact H2.
+Defined.
+
+Definition sle_n_m_S {n m} : sle n m -> sle (S n) (S m).
+Proof.
+  intros H. constructor;exact H.
 Defined.
 
 Definition sle_trans n m p (H : sle n m) (H': sle m  p) : sle n p.
@@ -70,7 +78,9 @@ Notation "# R" := (id_nat_hom R) (at level 70).
 
 Definition nat_comp (A B C : nat_obj) (g : B ≥ C) (f : A ≥ B) : nat_hom A C
   := sle_trans _ _ _ g f.
-Notation "f ∘ g" := (nat_comp _ _ _ f g) (at level 40).
+
+Notation "g ∘ f" := (nat_comp _ _ _ g f) (at level 40).
+
 
 Arguments sbox {_}.
 
@@ -96,69 +106,152 @@ Definition nat_cat : category :=
 
 (* The definition of [later] operator *)
 
-(* Building required context to pass to the tranlation
-   Maybe, we should try to use the template monad here *)
-
+(* Building required context to pass to the tranlation *)
 
 Quote Recursively Definition q_def := nat_hom.
 Definition g_ctx := fst q_def.
+Definition ΣE : tsl_context:= (reconstruct_global_context g_ctx,[]).
 
-Quote Definition qTypeConstr := (Type -> Type).
+Definition f_translate (cat : category) (tsl_ctx : tsl_context) (trm : term)
+  : tsl_result term :=
+  Success (snd (translate true None
+                          (snd tsl_ctx)
+                          cat
+                          ({| Environ.env_globals := (fst (fst tsl_ctx)) |})
+                          tt
+                          trm)).
 
-Definition tr_TypeConstr_syn :=
-  Eval vm_compute in
-    translate_type true None nil nat_cat
-                   {| Environ.env_globals := g_ctx|}
-                   tt qTypeConstr.
+Definition f_translate_type (cat : category) (tsl_ctx : tsl_context) (trm : term)
+  : tsl_result term :=
+  Success (snd (translate_type true None
+                               (snd tsl_ctx)
+                               cat
+                               ({| Environ.env_globals := (fst (fst tsl_ctx)) |})
+                               tt
+                               trm)).
 
-Import ListNotations.
+Definition ForcingTranslation (cat : category) : Translation :=
+  {| tsl_id := tsl_ident;
+     tsl_tm := f_translate cat;
+     tsl_ty := f_translate_type cat;
+     tsl_ind := fun _ _ _ _ => Error TranslationNotHandeled;
+     (* tsl_context -> kername -> kername -> mutual_inductive_body *)
+     (*             -> tsl_result (tsl_table * list mutual_inductive_body) *)
+  |}.
 
-Make Definition gTypeConstr := Eval vm_compute in (snd tr_TypeConstr_syn).
+Definition add_translation (ctx : tsl_context) (e : global_reference * term): tsl_context :=
+  let (Σ, E) := ctx in
+  (Σ, e :: E).
 
-Arguments nat_comp {_ _ _}.
+Instance GuardRec : Translation := ForcingTranslation nat_cat.
 
-Definition later : gTypeConstr.
-Proof.
-  unfold gTypeConstr.
-  intros p T q f.
-  destruct q.
+Import MonadNotation.
+Open Scope string_scope.
+
+Run TemplateProgram (tImplement ΣE "later" (Type->Type)).
+Next Obligation.
+  destruct p0.
   - apply unit.
-  - apply (T q (sle_Sn q ∘ f) q (# _)).
+  - apply (X p0 (sle_Sn p0 ∘ H) p0 (# _)).
 Defined.
 
-Quote Definition qType := Type.
+Notation "⊳ A" := (later A) (at level 40).
 
-Definition tr_Type_syn :=
+Quote Definition qL := laterᵗ.
+
+Definition ctx_with_later := add_translation ΣE  (ConstRef "Top.later", tConst "laterᵗ" []).
+
+Definition lArr := (fun (A B : Type) => ⊳ (A -> B)).
+
+Quote Definition qlArr := (fun (A B : Type) => ⊳ (A -> B)).
+
+Quote Definition qLapp := (forall A B (t : lArr A B) (u : ⊳ A), ⊳ B).
+
+Definition tr_LArr_syn :=
   Eval vm_compute in
-    translate_type true None nil nat_cat
+    translate true None [(ConstRef "Top.later", tConst "laterᵗ" [])] nat_cat
                    {| Environ.env_globals := g_ctx|}
-                   tt qType.
+                   tt qlArr.
 
-Make Definition gType := Eval vm_compute in (snd tr_Type_syn).
+(* Doesn't work because of the problems with universe levels *)
+(* Make Definition lArrᵗ := Eval vm_compute in (snd tr_LArr_syn). *)
 
-Definition later_type (A : gType) : gType
-  := fun p q α => later p (fun p' _ q' => A p' q') q α.
+(* We have to use lArr, otherwise we run into a problem with universe levels.
+   This is probably has to do with the fact that we do not generate a fresh universe variable in
+   the forcing transaltion of tSort, but reuse the previous level instead.*)
+Run TemplateProgram
+    ( TC <- tTranslate ΣE "lArr" ;;
+      (* TC <- tTranslateTm ctx_with_later "lArr" (fun (A B : Type) => ⊳ (A -> B)) ;; *)
+       tImplement TC "later_app"
+         (forall A B (t : lArr A B) (u : ⊳ A), ⊳ B)).
+Next Obligation.
+  destruct p.
+  - cbv. exact tt.
+  - simpl in *. specialize X with (p0:= S p) (α := (# _)).
+    simpl in X. apply X.
+    intros q β. specialize X0 with (p0:= S q) (α:= sle_n_m_S β).
+    simpl in X0. apply X0.
+Defined.
 
-Notation "⊳ A" := (later_type A) (at level 40).
+Notation "t ⊙ u" := (later_app _ _ t u) (at level 40).
 
-Quote Definition qId := (fun (A : Type) => A).
+Definition arrToLater := (fun T => T -> ⊳T).
 
-Definition tr_Arr_syn :=
-  Eval vm_compute in
-    translate true None nil nat_cat
-                   {| Environ.env_globals := g_ctx|}
-                   tt qId.
+(* Definition tr_nextp_syn := *)
+(*   Eval vm_compute in *)
+(*     translate_type true None [(ConstRef "Top.later", qL)] nat_cat *)
+(*                    {| Environ.env_globals := g_ctx|} *)
+(*                    tt q_nextp_ty. *)
 
-(*A translation of [fun (x : Type) => x] from the original plugin *)
-Definition fooᶠ  : forall p : nat_obj,
-    (forall p0 : nat_obj, p ≥ p0 -> forall p1 : nat_obj, p0 ≥ p1 -> Type) ->
-    forall p0 : nat_obj, p ≥ p0 -> Type
-  := (fun (p : nat_obj) (x : forall p0 : nat_obj, p ≥ p0 -> forall p1 : nat_obj, p0 ≥ p1 -> Type) => x p (# _)).
+(* Make Definition next_ty := Eval vm_compute in (snd tr_nextp_syn). *)
 
-Make Definition gId :=
-  Eval vm_compute in (snd tr_Arr_syn).
+Run TemplateProgram
+    ( TC <- tTranslate ΣE "arrToLater" ;;
+      tImplement TC "nextp" (forall {T:Type}, arrToLater T)).
+Next Obligation.
+  unfold arrToLaterᵗ. intros.
+  destruct p.
+  -  exact tt.
+  - simpl. refine (X p _).
+Defined.
 
-Lemma eq_gId_fooᶠ : gId = fooᶠ.
-Proof. reflexivity. Qed.
+Arguments functional_extensionality_dep {_ _} _ _ _.
 
-(* Definition later_app : forall A B (t : ⊳ (A -> B)) (u : ⊳ A), ⊳ B. *)
+(* We copy translated definitions of [eq] generated by the OCaml forcing plugin,
+   because inducives are not supported yet by template-coq forcing translation *)
+Inductive eqᵗ (p : nat_obj) (A : forall p0 : nat_obj, p ≥ p0 -> forall p : nat_obj, p0 ≥ p -> Type)
+(x : forall (p0 : nat_obj) (α : p ≥ p0), A p0 (α ∘ (# _)) p0 (# _))
+  : (forall (p0 : nat_obj) (α : p ≥ p0), A p0 ((# _) ∘ (α ∘ (# _))) p0 (# _)) -> Type :=
+  eq_reflᵗ : eqᵗ p A x x.
+
+
+(* We use this trick with η-expanded version of equiality to be able to use existing translations.
+   If we just lest plain [eq], the application would be of a special kind (of inductive type) and
+   it is translated differently, not as ordinary application of a global constant *)
+Definition eq_f {A: Type} (a b : A) : Prop := a = b.
+
+Definition eq_fᵗ := fun (p : nat_obj) (A : forall p0 : nat_obj, p ≥ p0 -> forall p1 : nat_obj, p0 ≥ p1 -> Type)
+  (a b : forall (p0 : nat_obj) (α : p ≥ p0), A p0 (α ∘ (# _)) p0 (# _)) (p0 : nat_obj)
+  (α : p ≥ p0) =>
+eqᵗ p0
+  (fun (p1 : nat_obj) (α0 : p0 ≥ p1) =>
+   (fun (p2 : nat_obj) (α1 : p ≥ p2) => A p2 (α1 ∘ (# _))) p1 ((# _) ∘ (α0 ∘ α)))
+  (fun (p1 : nat_obj) (α0 : p0 ≥ p1) =>
+   (fun (p2 : nat_obj) (α1 : p ≥ p2) => a p2 (α1 ∘ (# _))) p1 ((# _) ∘ (α0 ∘ α)))
+  (fun (p1 : nat_obj) (α0 : p0 ≥ p1) =>
+     (fun (p2 : nat_obj) (α1 : p ≥ p2) => b p2 (α1 ∘ (# _))) p1 ((# _) ∘ (α0 ∘ α))).
+
+
+Definition eq_is_eq : forall p A (x y: forall p0 (f:p ≥ p0), A p0 f p0 (# _)),
+    eq x y -> eqᵗ p _ x y.
+Proof.
+  intros. rewrite H. apply eq_reflᵗ.
+  (* Fails with the error "Bad relevance" *)
+Abort.
+
+(* If we remove this line, the definition for [next_id] fails because of universe levels *)
+Quote Definition qqq := (forall A u, eq_f (nextp _ (fun (x : A) => x) ⊙ u) u).
+
+Run TemplateProgram
+    (tImplement ΣE "next_id"  (forall A u, eq_f (nextp _ (fun (x : A) => x) ⊙ u) u)).
+Next Obligation. Admitted.
