forcing/Tests.v
@@ -1,0 +1,83 @@
+(* Some sanity tests for several definitions. We test agaist the tranlation acquired from the OCaml
+ forcing translation plugin (up to notation) *)
+Require Import Template.monad_utils Template.Ast
+        Template.Template Template.LiftSubst.
+Require Import String PeanoNat.
+Require Import Forcing.TemplateForcing.
+
+(* Some examples to play with  *)
+Definition Obj := Type.
+Definition Hom := (fun x y => x -> y).
+Notation "P ≥ Q" := (Hom P Q) (at level 70).
+
+Definition Id_hom := @id.
+Notation "# R" := (Id_hom R) (at level 70).
+
+Definition Comp := @Coq.Program.Basics.compose.
+Notation "g ∘ f" := (Comp _ _ _ g f) (at level 40).
+
+Definition test_cat : category :=
+  makeCatS "Obj" "Hom" "Id_hom" "Comp".
+
+
+Quote Recursively Definition q_def := Hom.
+Definition g_ctx := fst q_def.
+
+
+Quote Definition qId := (fun (A : Type) => A).
+
+Definition tr_Id_syn :=
+  Eval vm_compute in
+    translate true None nil test_cat
+                   {| Environ.env_globals := g_ctx|}
+                   tt qId.
+
+(*A translation of [fun (x : Type) => x] from the original plugin *)
+Definition fooᶠ  : forall p : Obj,
+    (forall p0 : Obj, p ≥ p0 -> forall p1 : Obj, p0 ≥ p1 -> Type) ->
+    forall p0 : Obj, p ≥ p0 -> Type
+  := (fun (p : Obj) (x : forall p0 : Obj, p ≥ p0 -> forall p1 : Obj, p0 ≥ p1 -> Type) => x p (# _)).
+
+Make Definition gId :=
+  Eval vm_compute in (snd tr_Id_syn).
+
+Lemma eq_gId_fooᶠ : gId = fooᶠ.
+Proof. reflexivity. Qed.
+
+
+Quote Definition qArr := (fun (A B : Type)  => A -> B).
+
+Definition tr_Arr_syn :=
+  Eval vm_compute in
+    translate true None nil test_cat
+                   {| Environ.env_globals := g_ctx|}
+                   tt qArr.
+
+
+(* Translation of [(fun (A B : Type)  => A -> B)] from the original plugin*)
+Definition barᶠ : forall p : Obj,
+    (forall p0 : Obj, p ≥ p0 -> forall p1 : Obj, p0 ≥ p1 -> Type) ->
+    (forall p0 : Obj, p ≥ p0 -> forall p1 : Obj, p0 ≥ p1 -> Type) ->
+    forall p0 : Obj, p ≥ p0 -> Type
+  := fun (p : Obj) (A B : forall p0 : Obj, p ≥ p0 -> forall p1 : Obj, p0 ≥ p1 -> Type)
+         (p0 : Obj) (α : p ≥ p0) =>
+       (forall (p1 : Obj) (α0 : p0 ≥ p1), A p1 ((# _) ∘ (α0 ∘ α)) p1 (# _)) -> B p0 (α ∘ (# _)) p0 (# _).
+
+Make Definition bar := Eval vm_compute in (snd tr_Arr_syn).
+
+Lemma eq_bar_barᶠ : bar = barᶠ.
+Proof.
+  reflexivity.
+Qed.
+
+Quote Definition bazz :=  (forall (A : Type), (A -> Type)).
+
+Definition tr_bazz_syn :=
+  Eval vm_compute in
+    translate_type true None nil test_cat
+                   {| Environ.env_globals := g_ctx|}
+                   tt bazz.
+
+(* Just testing that the definition can be reflected back from quoted. This covers a bug with
+   top-level condition variable when building a chain of moprhisms by composition *)
+Make Definition bazz' := Eval vm_compute in (snd tr_bazz_syn).
